theory/readwrite.v
@@ -1,0 +1,35 @@
+Require Import Unicode.Utf8.
+Require Import syntax semantics util.
+Require Import List.
+Import ListNotations.
+
+Definition read_write x y t T r :=
+  elet x t (read (id y)) 
+    (write (new T r) (id x)).
+
+Lemma read_write_ordering : ∀ x y l t T r v l',
+  ([(r, [l'])], [(y, vl l)], [], [(l,v)], [], new T r) ↦ (vl l', []) →
+  ([(r, [l'])], [(y, vl l)], [], [(l,v)], [], read_write x y t T r) ↦ (vl l', [mwrite l' v; mread l v]).
+Proof.
+intros. apply ELet with (v0:=v) (E:=[mread l v]) (S:=[(l,v)])
+                        (S':=[(l,v)]) (E':=[mwrite l' v]). 
+  - assert ([mread l v] = [] ++ [mread l v]).  symmetry. apply app_nil_l. rewrite H0. 
+    constructor. constructor. apply lookup_cons. auto. apply lookup_cons. 
+  - simpl.  reflexivity.  
+  - assert ([mwrite l' v] = [] ++ [mwrite l' v]). rewrite
+    <- app_nil_l. reflexivity. rewrite H0. apply EWrite with (S':=[(l,v)])
+    (E1:=[]) (E2:=[]). 
+    + constructor. 
+      * unfold lu. rewrite lookup_cons. constructor. reflexivity.  
+      * inversion H. subst. assumption. 
+    + constructor. apply lookup_cons. 
+    + constructor. constructor. intros; auto. inversion H1; auto. 
+      inversion H2; auto. inversion H3.  reflexivity. 
+  - constructor. assert ([[mread l v] ; [mwrite l' v]] = ([[mread l v]] ++
+    ([mwrite l' v ]) :: [])). auto. rewrite H0. constructor. simpl. assert
+    ([[mread l v]; []] = [] ++ [mread l v] :: [[]]). reflexivity. rewrite H1.
+    constructor. constructor. intros. simpl in *. destruct H2; auto. destruct
+    H2; auto. inversion H2. reflexivity. 
+Qed.
+
+
